

$$1. a) E[X] = \frac{1}{6} (1+2+3+4+5+6) = \frac{21}{6}$$

$$b) E[X] = \frac{1}{36} (2) + \frac{2}{36} (3) + \frac{3}{36} (4) + \frac{4}{36} (5) \\ + \frac{6}{36} (7) + \frac{5}{36} (8) + \frac{4}{36} (9) + \frac{3}{36} (10) \\ + \frac{2}{36} (11) + \frac{1}{36} (12) = \frac{252}{36}$$

c) k slots, so $\frac{k}{37}$ prob of winning

$$E[X] = \frac{k}{37} \left(\frac{36}{k} \right) + \frac{37-k}{37} (0) - 1 \\ = \frac{36}{37} - 1$$

$$d) \frac{1}{6} (1+2+5+4+5) + \frac{1}{6} (6) + \frac{1}{6} (1+2+3+4+5+6) \\ = \frac{24.5}{6}$$

e) Recursive, so

$$R = \frac{1}{6} (1+2+3+4+5) + \frac{1}{6} (6+R) \\ = \frac{21}{6} + \frac{R}{6} \Rightarrow 4.2$$

$$3. a) \int_0^1 (x-0.5)^2 dx = \int_0^1 x^2 - x + 0.25 dx$$

$$= \left. \frac{1}{3} x^3 - \frac{1}{2} x^2 + 0.25 x \right|_0^1 = \frac{1}{3} - \frac{1}{2} + \frac{1}{4} = \left(\frac{1}{12} \right)$$

$$b) V[X] = \int (x - E[X])^2 f(x) dx$$

$$= \int (x^2 - 2xE[X] + E[X]^2) f(x) dx$$

$$= \int x^2 f(x) dx - \int 2xE[X] f(x) dx + \int E[X]^2 f(x) dx$$

$$= E[X^2] - 2E[X]^2 + E[X]^2$$

$$= E[X^2] - E[X]^2$$

$$c) V[a+bX] = \int (a+bX - E[a+bX])^2 f(x) dx$$

$$= \int (a+bX - a - bE[X])^2 f(x) dx$$

$$= \int b^2 (X - E[X])^2 f(x) dx$$

$$= b^2 \int (X - E[X])^2 f(x) dx$$

$$= b^2 V[X] \checkmark$$

$$d) f_x\left(\frac{y-\mu}{\sigma}\right) = \int_{-\infty}^{\infty} \frac{1}{\sigma} \exp\left\{-\frac{1}{2}\left(\frac{(y-\mu)(t-\mu)}{\sigma}\right)^2\right\}$$

$$\text{form of norm dist} \Rightarrow \int_{-\infty}^{\infty} \frac{1}{\sqrt{2\pi}} \exp\left\{-\frac{1}{2}\left(\frac{y-\mu'}{\sigma'}\right)^2\right\} dx$$

$$4. a) \text{cov}(x, y) = \int_y \int_x (x - E[x])(y - E[y]) f_x(x) f_y(y) dx dy$$

$$= \int_y \left[\int_x x f_x(x) dx - E[x] \right] (y - E[y]) f_y(y) dy$$

$$= \int_y [0] (y - E[y]) f_y(y) dy$$

$$= 0$$

b) Simulation in code file

$$5. a) E[\varepsilon] = \int (x - E[x]) f(x) dx$$

$$= \int x f(x) dx - E[x]$$

$$= 0$$

$$\begin{aligned}
 b) \quad V[\epsilon] &= \int (x - E[x] - E[x - E[x]])^2 f(x) dx \\
 &= \int (x - E[x] - 0)^2 f(x) dx \\
 &= V[x]
 \end{aligned}$$

$$\begin{aligned}
 c) \quad E[x] &= E[E[x]] + E[\sigma_x \epsilon] \\
 &= E[x] + \sigma_x E[\epsilon] \\
 &= E[x] + \sigma_x 0 \\
 &= E[x]
 \end{aligned}$$

$$\begin{aligned}
 d) \quad V[x] &= \int E[x] + \sigma_x \epsilon - E[E[x] + \sigma_x \epsilon]^2 f(x) dx \\
 &= \int [E[x] + \sigma_x \epsilon - E[x] - \sigma_x E[\epsilon]]^2 f(x) dx \\
 &= \int (\sigma_x \epsilon - \sigma_x E[\epsilon])^2 f(x) dx \\
 &= \int \sigma_x^2 (\epsilon - E[\epsilon])^2 f(x) dx \\
 &= \sigma_x^2 \int (\epsilon - E[\epsilon])^2 f(x) dx \\
 &= \sigma_x^2 V[\epsilon] = \sigma_x^2
 \end{aligned}$$

$$6. \quad E[f_{x,h}(x)] = \frac{F(x+h) - F(x-h)}{2h}$$

$$\begin{aligned} \text{So} \quad & \frac{F(x) + hC f(x) + \frac{1}{2} h^2 f'(x) + o(h^3) - F(x)}{2h} \\ & + \frac{h f(x) - \frac{1}{2} h^2 f'(x) - o(h^3)}{2h} \end{aligned}$$

$$\Rightarrow 2h f(x) + o(h^3) + h f(x) - o(h^3)$$

$$\Rightarrow \underline{f(x) + o(h^2)}$$